update after presentation

Demo/Demo.lean
@@ -3,24 +3,59 @@ import Mathlib.Tactic.Ring
 import Std
 import Demo.Util
 
-def fib : Nat → Nat := sorry
+def fib : Nat → Nat
+  | 0 => 0
+  | 1 => 1
+  | n + 2 => fib (n + 1) + fib n
 
--- set_option trace.Meta.Tactic.simp.rewrite true in
--- theorem fib_add_two {n : ℕ} : fib (n + 2) = fib n + fib (n + 1) := by
---   simp [fib, add_comm]
+#eval fib 15
+#eval List.map fib (List.range 20)
+
+--set_option trace.Meta.Tactic.simp.rewrite true in
+theorem fib_add_two {n : ℕ} : fib (n + 2) = fib n + fib (n + 1) := by
+  simp [fib, add_comm]
 
 lemma fib_add (m n : ℕ) :
     fib (m + n + 1) = fib m * fib n + fib (m + 1) * fib (n + 1) := by
-  sorry
+  induction n generalizing m
+  case zero =>
+    simp [fib]
+  case succ n ih =>
+    specialize ih (m + 1)
+    rw [add_assoc m 1 n, add_comm 1 n] at ih
+    simp only [fib_add_two, ih]
+    ring
 
-def fib₀ : Nat → Nat := sorry
+def fib₀ : Nat → Nat
+  | 0 => 0
+  | n + 1 => (aux n).2
+where
+  aux : Nat → Nat × Nat
+    | 0 => (0, 1)
+    | n + 1 =>
+      let (a, b) := aux n
+      (b, a + b)
 
--- lemma fib₀_aux_eq (n : Nat) : fib₀.aux n = (fib n, fib (n + 1)) := by
+#eval fib₀ 1000
+
+lemma fib₀_aux_eq (n : Nat) : fib₀.aux n = (fib n, fib (n + 1)) := by
+  induction n
+  . simp [fib]
+  . next _ ih => simp [fib₀.aux, fib, ih, add_comm]
+
+@[csimp] theorem fib_eq : fib = fib₀ := by
+  ext n
+  cases n <;> simp [fib, fib₀, fib₀_aux_eq, add_comm]
+
+#eval fib 1000
 
 def fib₁ (n : Nat) :=
   aux n 0 1
-where aux : Nat → Nat → Nat → Nat := sorry
+where aux : Nat → Nat → Nat → Nat
+  | 0, _, b => b
+  | n+1, a, b => aux n b (a + b)
 
+#eval fib₁ 400000
 -- #eval fib₁ 400000
 
 def fib₂ (n : Nat) : Nat := Id.run do
@@ -30,20 +65,42 @@ def fib₂ (n : Nat) : Nat := Id.run do
     p := (b, a + b)
   return p.1
 
+#eval fib₂ 100
+
+def fib₃ (n : Nat) : Nat := Id.run do
+  let mut a := 0
+  let mut b := 1
+  for _ in [:n] do
+    let temp := a
+    a := b
+    b := temp + b
+  return b
+
 def fib₄ (n : Nat) : { m // m = fib n } :=
   let ⟨pair, property⟩ :=
   loop_with_invariant
-    (invariant := sorry)
+    (invariant := fun i p => p = (fib i, fib (i + 1)))
     (start_state := (0, 1))
-    (init := sorry)
+    (init := by simp [fib])
     (next_state := fun i p =>
-      sorry)
-    (step := sorry)
+      let (a, b) := p
+      (b, a + b))
+    (step := by intro i; simp [fib, add_comm])
     n
-  sorry
+  ⟨pair.1, by simp [property]⟩
 
-def fib₅ (n : Nat) : { m // m = fib n } := sorry
+#eval fib₄ 10000
 
+def fib₅ (n : Nat) : { m // m = fib n } :=
+  for i upto n
+    state: p := (0, 1)
+    invariant: inv := p = (fib i, fib (i + 1))
+    init:= by simp
+    next:
+      let (a, b) := p
+      (b, a + b)
+    step:= by intro i; simp [fib, add_comm]
+  ⟨p.1, by simp [inv]⟩
 
 /-
 Notes.
@@ -73,7 +130,7 @@ Thesis: we should be able to simulate the functionality of e.g. Dafny.
 -/
 
 -- set_option trace.Meta.Tactic.simp true in
--- set_option trace.Meta.synthInstance true in
+set_option trace.Meta.synthInstance true in
 example : (x + 2) + 2 = x + 4 := by simp [add_assoc]
 
 #check add_assoc
